theories/binary_format_printer.v
@@ -1,0 +1,153 @@
+Require Import datatypes_properties numerics.
+From compcert Require Import Integers.
+From parseque Require Import Parseque.
+Require Import Ascii Byte.
+Require Import leb128.
+Require Import Coq.Arith.Le.
+From mathcomp Require Import ssreflect ssrfun ssrnat ssrbool eqtype seq.
+
+Definition binary_of_value_type (t : value_type) : byte :=
+  match t with
+  | T_i32 => x7f
+  | T_i64 => x7e
+  | T_f32 => x7d
+  | T_f64 => x7c
+  end.
+
+Definition binary_of_block_type_aux (bt : list value_type) : list byte :=
+  match bt with
+  | nil => x40 :: nil
+  | cons t nil => binary_of_value_type t :: nil
+  | _ => (* TODO: this should never occur *) nil
+  end.
+
+Definition binary_of_block_type (ft : function_type) : list byte :=
+  match ft with
+  | Tf nil rt => binary_of_block_type_aux rt
+  | _ => (* TODO: should never happen *) nil
+  end.
+
+Definition binary_of_u32_nat (n : nat) :=
+  List.map (byte_of_ascii) (encode_unsigned (BinNatDef.N.of_nat n)).
+
+Definition binary_of_idx n := binary_of_u32_nat n.
+
+Definition binary_of_vec {A} (f : A -> list byte) (es : list A) : list byte :=
+  (binary_of_u32_nat (List.length es)) ++ (List.concat (List.map f es)).
+
+Definition binary_of_memarg a o : list byte :=
+binary_of_u32_nat a ++ binary_of_u32_nat o.
+
+Definition binary_of_i32 (x : i32) : list byte :=
+  (* TODO *)
+  x00 :: x00 :: x00 :: nil.
+
+Definition binary_of_i64 (x : i64) : list byte :=
+  (* TODO *)
+  x00 :: x00 :: x00 :: nil.
+
+Definition binary_of_f32 (x : f32) : list byte :=
+  (* TODO *)
+  x00 :: x00 :: x00 :: nil.
+
+Definition binary_of_f64 (x : f64) : list byte :=
+  (* TODO *)
+  x00 :: x00 :: x00 :: nil.
+
+Fixpoint binary_of_be (be : basic_instruction) : list byte :=
+  let binary_of_instrs bes := List.concat (List.map binary_of_be bes) in
+  match be with
+  | Unreachable => x00 :: nil
+  | Nop => x01 :: nil
+  | Block rt ins =>
+    (x02 :: nil) ++ binary_of_block_type rt ++ binary_of_instrs ins ++ (x0b :: nil)
+  | Loop rt ins =>
+    (x03 :: nil) ++ binary_of_block_type rt ++ binary_of_instrs ins ++ (x0b :: nil)
+  | If rt ins nil =>
+    (x04 :: nil) ++ binary_of_block_type rt ++ binary_of_instrs ins ++ (x0b :: nil)
+  | If rt ins1 ins2 =>
+    (x04 :: nil) ++ binary_of_block_type rt ++ binary_of_instrs ins1 ++ (x05 :: nil) ++ binary_of_instrs ins2 ++ (cons x0b nil)
+  | Br l => x0c :: binary_of_idx l
+  | Br_if l => x0d :: binary_of_idx l
+  | Br_table ls l_N =>
+    x0e :: ((binary_of_vec binary_of_idx ls) ++ binary_of_idx l_N)
+  | Return => x0f :: nil
+  | Call x => x10 :: binary_of_idx x
+  | Call_indirect x => x11 :: (binary_of_idx x ++ (x00 :: nil))
+  | Drop => x1a :: nil
+  | Select => x1b :: nil
+  | Get_local x => x20 :: binary_of_idx x
+  | Set_local x => x21 :: binary_of_idx x
+  | Tee_local x => x22 :: binary_of_idx x
+  | Get_global x => x23 :: binary_of_idx x
+  | Set_global x => x24 :: binary_of_idx x
+  | Load T_i32 None a o => x28 :: binary_of_memarg a o
+  | Load T_i64 None a o => x29 :: binary_of_memarg a o
+  | Load T_f32 None a o => x2a :: binary_of_memarg a o
+  | Load T_f64 None a o => x2b :: binary_of_memarg a o
+  | Load T_i32 (Some (Tp_i8, sx_S)) a o => x2c :: binary_of_memarg a o
+  | Load T_i32 (Some (Tp_i8, sx_U)) a o => x2d :: binary_of_memarg a o
+  | Load T_i32 (Some (Tp_i16, sx_S)) a o => x2e :: binary_of_memarg a o
+  | Load T_i32 (Some (Tp_i16, sx_U)) a o => x2f :: binary_of_memarg a o
+  | Load T_i64 (Some (Tp_i8, sx_S)) a o => x30 :: binary_of_memarg a o
+  | Load T_i64 (Some (Tp_i8, sx_U)) a o => x31 :: binary_of_memarg a o
+  | Load T_i64 (Some (Tp_i16, sx_S)) a o => x32 :: binary_of_memarg a o
+  | Load T_i64 (Some (Tp_i16, sx_U)) a o => x33 :: binary_of_memarg a o
+  | Load T_i64 (Some (Tp_i32, sx_S)) a o => x34 :: binary_of_memarg a o
+  | Load T_i64 (Some (Tp_i32, sx_U)) a o => x35 :: binary_of_memarg a o
+  | Store T_i32 None a o => x36 :: binary_of_memarg a o
+  | Store T_i64 None a o => x37 :: binary_of_memarg a o
+  | Store T_f32 None a o => x38 :: binary_of_memarg a o
+  | Store T_f64 None a o => x39 :: binary_of_memarg a o
+  | Store T_i32 (Some Tp_i8) a o => x3a :: binary_of_memarg a o
+  | Store T_i32 (Some Tp_i16) a o => x3b :: binary_of_memarg a o
+  | Store T_i64 (Some Tp_i8) a o => x3c :: binary_of_memarg a o
+  | Store T_i64 (Some Tp_i16) a o => x3d :: binary_of_memarg a o
+  | Store T_i64 (Some Tp_i32) a o => x3e :: binary_of_memarg a o
+  | Current_memory => x3f :: x00 :: nil
+  | Grow_memory => x40 :: x00 :: nil
+  | EConst (ConstInt32 x) => x41 :: binary_of_i32 x
+  | EConst (ConstInt64 x) => x42 :: binary_of_i64 x
+  | EConst (ConstFloat32 x) => x43 :: binary_of_f32 x
+  | EConst (ConstFloat64 x) => x44 :: binary_of_f64 x
+  | Testop T_i32 Eqz => x45 :: nil
+  | Relop_i T_i32 Eq => x46 :: nil
+  | Relop_i T_i32 Ne => x47 :: nil
+  | Relop_i T_i32 (Lt sx_S) => x48 :: nil
+  | Relop_i T_i32 (Lt sx_U) => x49 :: nil
+  | Relop_i T_i32 (Gt sx_S) => x4a :: nil
+  | Relop_i T_i32 (Gt sx_U) => x4b :: nil
+  | Relop_i T_i32 (Le sx_S) => x4c :: nil
+  | Relop_i T_i32 (Le sx_U) => x4d :: nil
+  | Relop_i T_i32 (Ge sx_S) => x4e :: nil
+  | Relop_i T_i32 (Ge sx_U) => x4f :: nil
+  | Testop T_i64 Eqz => x50 :: nil
+  | Relop_i T_i64 Eq => x51 :: nil
+  | Relop_i T_i64 Ne => x52 :: nil
+  | Relop_i T_i64 (Lt sx_S) => x53 :: nil
+  | Relop_i T_i64 (Lt sx_U) => x54 :: nil
+  | Relop_i T_i64 (Gt sx_S) => x55 :: nil
+  | Relop_i T_i64 (Gt sx_U) => x56 :: nil
+  | Relop_i T_i64 (Le sx_S) => x57 :: nil
+  | Relop_i T_i64 (Le sx_U) => x58 :: nil
+  | Relop_i T_i64 (Ge sx_S) => x59 :: nil
+  | Relop_i T_i64 (Ge sx_U) => x5a :: nil
+  | Relop_f T_f32 Eqf => x5b :: nil
+  | Relop_f T_f32 Nef => x5c :: nil
+  | Relop_f T_f32 Ltf => x5d :: nil
+  | Relop_f T_f32 Gtf => x5e :: nil
+  | Relop_f T_f32 Lef => x5f :: nil
+  | Relop_f T_f32 Gef => x60 :: nil
+  | Relop_f T_f64 Eqf => x61 :: nil
+  | Relop_f T_f64 Nef => x62 :: nil
+  | Relop_f T_f64 Ltf => x63 :: nil
+  | Relop_f T_f64 Gtf => x64 :: nil
+  | Relop_f T_f64 Lef => x65 :: nil
+  | Relop_f T_f64 Gef => x66 :: nil
+
+  | _ => (* TODO: deal with all the other cases *) x00 :: x00 :: x00 :: nil
+  end.
+
+Definition binary_of_module (m : module) : list byte :=
+  (* TODO *)
+  nil.
