theories/binary_format_spec.v
@@ -1,4 +1,4 @@
-From Wasm Require Import datatypes_properties.
+From Wasm Require Import datatypes_properties binary_format_parser binary_format_printer.
 From compcert Require Import Integers.
 From parseque Require Import Parseque.
 Require Import Ascii Byte.
@@ -11,5 +11,11 @@ Inductive repr_unsigned : list ascii -> module -> Prop :=
 Inductive repr_module : list ascii -> module -> Prop :=
 .
 
-(* TODO: we have ast->binary->ast = id
+(* TODO: we should have ast->binary->ast = id
    but not binary->ast->binary /= id, because of non-unique representation  *)
+
+Lemma encode_decode_is_identity : forall m,
+(* TODO: probably need some well-formedness condition, for example of block types *)
+  parse_module_from_bytes (binary_of_module m) = Some m.
+(* TODO *)
+Admitted.
