theories/binary_format_tests.v
@@ -1,0 +1,354 @@
+(** Tests for the binary parser. **)
+Require Import Coq.Strings.String.
+Open Scope string_scope.
+Require Import Byte.
+
+(* for pretty-printing *)
+Definition hex_small_no_prefix_of_byte (b : byte) :=
+(*
+#!/usr/bin/env ocaml
+open Char
+let a_code = Char.code 'a'
+let show = function
+| x when x < 10 -> string_of_int x
+| x -> String.make 1 (Char.chr (a_code + x - 10))
+let _ =
+for i = 0 to 15 do
+for j = 0 to 15 do
+let x = show i in
+let y = show j in
+print_string ("| x" ^ x ^ y ^ " => \"" ^ x ^ y ^ "\"\n")
+done
+done
+*)
+match b with
+| x00 => "00"
+| x01 => "01"
+| x02 => "02"
+| x03 => "03"
+| x04 => "04"
+| x05 => "05"
+| x06 => "06"
+| x07 => "07"
+| x08 => "08"
+| x09 => "09"
+| x0a => "0a"
+| x0b => "0b"
+| x0c => "0c"
+| x0d => "0d"
+| x0e => "0e"
+| x0f => "0f"
+| x10 => "10"
+| x11 => "11"
+| x12 => "12"
+| x13 => "13"
+| x14 => "14"
+| x15 => "15"
+| x16 => "16"
+| x17 => "17"
+| x18 => "18"
+| x19 => "19"
+| x1a => "1a"
+| x1b => "1b"
+| x1c => "1c"
+| x1d => "1d"
+| x1e => "1e"
+| x1f => "1f"
+| x20 => "20"
+| x21 => "21"
+| x22 => "22"
+| x23 => "23"
+| x24 => "24"
+| x25 => "25"
+| x26 => "26"
+| x27 => "27"
+| x28 => "28"
+| x29 => "29"
+| x2a => "2a"
+| x2b => "2b"
+| x2c => "2c"
+| x2d => "2d"
+| x2e => "2e"
+| x2f => "2f"
+| x30 => "30"
+| x31 => "31"
+| x32 => "32"
+| x33 => "33"
+| x34 => "34"
+| x35 => "35"
+| x36 => "36"
+| x37 => "37"
+| x38 => "38"
+| x39 => "39"
+| x3a => "3a"
+| x3b => "3b"
+| x3c => "3c"
+| x3d => "3d"
+| x3e => "3e"
+| x3f => "3f"
+| x40 => "40"
+| x41 => "41"
+| x42 => "42"
+| x43 => "43"
+| x44 => "44"
+| x45 => "45"
+| x46 => "46"
+| x47 => "47"
+| x48 => "48"
+| x49 => "49"
+| x4a => "4a"
+| x4b => "4b"
+| x4c => "4c"
+| x4d => "4d"
+| x4e => "4e"
+| x4f => "4f"
+| x50 => "50"
+| x51 => "51"
+| x52 => "52"
+| x53 => "53"
+| x54 => "54"
+| x55 => "55"
+| x56 => "56"
+| x57 => "57"
+| x58 => "58"
+| x59 => "59"
+| x5a => "5a"
+| x5b => "5b"
+| x5c => "5c"
+| x5d => "5d"
+| x5e => "5e"
+| x5f => "5f"
+| x60 => "60"
+| x61 => "61"
+| x62 => "62"
+| x63 => "63"
+| x64 => "64"
+| x65 => "65"
+| x66 => "66"
+| x67 => "67"
+| x68 => "68"
+| x69 => "69"
+| x6a => "6a"
+| x6b => "6b"
+| x6c => "6c"
+| x6d => "6d"
+| x6e => "6e"
+| x6f => "6f"
+| x70 => "70"
+| x71 => "71"
+| x72 => "72"
+| x73 => "73"
+| x74 => "74"
+| x75 => "75"
+| x76 => "76"
+| x77 => "77"
+| x78 => "78"
+| x79 => "79"
+| x7a => "7a"
+| x7b => "7b"
+| x7c => "7c"
+| x7d => "7d"
+| x7e => "7e"
+| x7f => "7f"
+| x80 => "80"
+| x81 => "81"
+| x82 => "82"
+| x83 => "83"
+| x84 => "84"
+| x85 => "85"
+| x86 => "86"
+| x87 => "87"
+| x88 => "88"
+| x89 => "89"
+| x8a => "8a"
+| x8b => "8b"
+| x8c => "8c"
+| x8d => "8d"
+| x8e => "8e"
+| x8f => "8f"
+| x90 => "90"
+| x91 => "91"
+| x92 => "92"
+| x93 => "93"
+| x94 => "94"
+| x95 => "95"
+| x96 => "96"
+| x97 => "97"
+| x98 => "98"
+| x99 => "99"
+| x9a => "9a"
+| x9b => "9b"
+| x9c => "9c"
+| x9d => "9d"
+| x9e => "9e"
+| x9f => "9f"
+| xa0 => "a0"
+| xa1 => "a1"
+| xa2 => "a2"
+| xa3 => "a3"
+| xa4 => "a4"
+| xa5 => "a5"
+| xa6 => "a6"
+| xa7 => "a7"
+| xa8 => "a8"
+| xa9 => "a9"
+| xaa => "aa"
+| xab => "ab"
+| xac => "ac"
+| xad => "ad"
+| xae => "ae"
+| xaf => "af"
+| xb0 => "b0"
+| xb1 => "b1"
+| xb2 => "b2"
+| xb3 => "b3"
+| xb4 => "b4"
+| xb5 => "b5"
+| xb6 => "b6"
+| xb7 => "b7"
+| xb8 => "b8"
+| xb9 => "b9"
+| xba => "ba"
+| xbb => "bb"
+| xbc => "bc"
+| xbd => "bd"
+| xbe => "be"
+| xbf => "bf"
+| xc0 => "c0"
+| xc1 => "c1"
+| xc2 => "c2"
+| xc3 => "c3"
+| xc4 => "c4"
+| xc5 => "c5"
+| xc6 => "c6"
+| xc7 => "c7"
+| xc8 => "c8"
+| xc9 => "c9"
+| xca => "ca"
+| xcb => "cb"
+| xcc => "cc"
+| xcd => "cd"
+| xce => "ce"
+| xcf => "cf"
+| xd0 => "d0"
+| xd1 => "d1"
+| xd2 => "d2"
+| xd3 => "d3"
+| xd4 => "d4"
+| xd5 => "d5"
+| xd6 => "d6"
+| xd7 => "d7"
+| xd8 => "d8"
+| xd9 => "d9"
+| xda => "da"
+| xdb => "db"
+| xdc => "dc"
+| xdd => "dd"
+| xde => "de"
+| xdf => "df"
+| xe0 => "e0"
+| xe1 => "e1"
+| xe2 => "e2"
+| xe3 => "e3"
+| xe4 => "e4"
+| xe5 => "e5"
+| xe6 => "e6"
+| xe7 => "e7"
+| xe8 => "e8"
+| xe9 => "e9"
+| xea => "ea"
+| xeb => "eb"
+| xec => "ec"
+| xed => "ed"
+| xee => "ee"
+| xef => "ef"
+| xf0 => "f0"
+| xf1 => "f1"
+| xf2 => "f2"
+| xf3 => "f3"
+| xf4 => "f4"
+| xf5 => "f5"
+| xf6 => "f6"
+| xf7 => "f7"
+| xf8 => "f8"
+| xf9 => "f9"
+| xfa => "fa"
+| xfb => "fb"
+| xfc => "fc"
+| xfd => "fd"
+| xfe => "fe"
+| xff => "ff"
+end.
+
+Require Import binary_format_parser binary_format_printer.
+Require Import datatypes_properties.
+From parseque Require Import Parseque Running.
+Require Import check_toks.
+
+Lemma test_unreachable : check_toks (x00 :: nil) be = Singleton Unreachable.
+Proof. reflexivity. Qed.
+
+Lemma test_nop : check_toks (x01 :: nil) be = Singleton Nop.
+Proof. reflexivity. Qed.
+
+Definition plop (x : list Byte.byte) :=
+  String.concat " " (List.map hex_small_no_prefix_of_byte x).
+
+Compute plop (binary_of_be (If (Tf nil nil) (Testop T_i64 Eqz :: nil) (Testop T_i64 Eqz :: nil))).
+
+Definition test2 : list Byte.byte :=
+  x04 :: x40
+  :: x50
+  :: x05
+  :: x50
+  :: x0b
+  :: x0b
+  :: nil.
+
+Compute parse_expr_from_bytes test2.
+
+(** Example from Wikipedia: https://en.wikipedia.org/wiki/WebAssembly#Code_representation
+  This is the representation of a factorial function. **)
+Definition test_wikipedia : list Byte.byte :=
+  x20 :: x00
+  :: x50
+  :: x04 :: x7e
+  :: x42 :: x01
+  :: x05
+  :: x20 :: x00
+  :: x20 :: x00
+  :: x42 :: x01
+  :: x7d
+  :: x10 :: x00
+  :: x7e
+  :: x0b
+  :: nil.
+
+Compute parse_expr_from_bytes test_wikipedia.
+
+(*
+Definition test_factorial :=
+  Block (
+    Get_local 0
+    :: Get_local 0
+    :: Testop T_i64 Eqz
+    (* TODO: continue the translation: I don’t know how to encode this. *)
+if (result i64)
+    i64.const 1
+else
+    local.get 0
+    local.get 0
+    i64.const 1
+    i64.sub
+    call 0
+    i64.mul
+end
+*)
+
+(* TODO: The parser fails here! So either Wikipedia is wrong (and we have to update the article),
+  or the parser is (and we have to update it) ☺
+Lemma test_wikipedia_correct : check_toks test_wikipedia be = Singleton test_factorial.
+Proof.
+  reflexivity.
+Qed.
+*)
