theories/extraction.v
@@ -1,9 +1,9 @@
 (** Extraction to OCaml. **)
 (* (C) M. Bodin - see LICENSE.txt *)
 
-From Wasm Require Import binary_parser type_checker interpreter.
+From Wasm Require Import binary_format_parser type_checker interpreter.
 
 Extraction Language OCaml.
 
-Extraction "extract" parse_wasm cl_type_check run_v.
+Extraction "extract" parse_be cl_type_check run_v.
 
